% \input{\pSections sec-derivation}

\section{Derivation}
\label{sec:derive}
		%

%     %     %     %     %     %     %     %     %
\subsection{Orbit Equation}
\begin{equation}
	\frac{d u^{2}}{d^{2} \lambda} + u = \frac{\mu}{h}, \quad u(0) = u_{0}, u'(0) = v_{0}
\label{eq:forced-oscillator}
\end{equation}
		%
A second order linear partial differential equation \cite{boyce2021elementary}
		%
First find the solution for the homogenous equation
		%
\begin{equation}
	\frac{d u^{2}}{d^{2} \lambda} + u =0
\label{eq:unforced-oscillator}
\end{equation}
		%
which is
			%
\begin{equation}
	u(\theta) = A \cos \theta + B \sin \theta
\label{eq:homogenous}
\end{equation}
		%
Using the boundary conditions, $u(\theta) = u_{0} \cos \theta + v_{0} \sin \theta$.

%     %     %     %     %     %     %     %     %
\subsection{Ellipse}
		%
\begin{equation}
	\frac{ \xi^{2} } { a^{2} } + \frac{ \eta^{2} } { b^{2} } = 1
\label{eq:derive:ellipse}
\end{equation}
		%
\begin{equation}
	\xi = ae + r\cos f, \eta = r\sin f, b^{2} = a^{2}(1 - e^{2})
\label{eq:derive:subs}
\end{equation}
		%
\begin{equation}
	(1 - e^{2}) \xi^{2} + \eta^{2} - a^{2}(1 - e^{2}) = 0
\label{eq:derive:new-quad}
\end{equation}
		%
\begin{equation}
	f(r) = \alpha r^{2} + \beta r + \gamma = 0
\label{eq:derive:see-quad}
\end{equation}
		%
\begin{equation}
	\alpha = 1 - e^{2} \cos^{2} f, \quad \beta = 2ae (1 - e^{2})\cos f, \quad \gamma = a^{2}(1 - e^{2})^{2}
\label{eq:derive:terms-quad}
\end{equation}
		%
\begin{equation}
	r_{\pm} = \frac{ -\beta \pm \sqrt{ \beta^{2} - 4 \alpha \gamma}} { 2\alpha }
\label{eq:derive:roots-quad}
\end{equation}
		%
\begin{equation}
	r_{+} = \frac{ a(1 - e^{2}) } { 1 + e \cos f }, \quad r_{-} = \frac{ -a(1 - e^{2}) } { 1 - e \cos f }
\label{eq:derive:roots-quad}
\end{equation}


\endinput  %  ==  ==  ==  ==  ==  ==  ==  ==  ==
